Phi_Semantics/PhiSem_Int_ArbiPrec.thy
@@ -202,7 +202,7 @@ lemma op_const_aint_\<phi>app[\<phi>synthesis 300]:
   by (rule, simp add: \<phi>expns)
 
 lemma op_const_anat_\<phi>app[\<phi>synthesis 300]:
-  \<open> \<^bold>s\<^bold>i\<^bold>m\<^bold>p\<^bold>l\<^bold>i\<^bold>f\<^bold>y x' : of_nat x \<comment>\<open>TODO: improve this!\<close>
+  \<open> \<s>\<i>\<m>\<p>\<l>\<i>\<f>\<y> x' : of_nat x \<comment>\<open>TODO: improve this!\<close>
 \<Longrightarrow> Check_Literal x'
 \<Longrightarrow> \<p>\<r>\<o>\<c> op_const_aint x' \<lbrace> Void \<longmapsto> \<v>\<a>\<l> x \<Ztypecolon> \<nat> \<rbrace>\<close>
   \<medium_left_bracket> op_const_aint[where x=x'] \<medium_right_bracket>. .
