Phi_System/IDE_CP_Reasoning1.thy
@@ -153,7 +153,8 @@ structure Assertion_SS_Abnormal = Simpset (
       Raw_Simplifier.merge_ss (Assertion_SS.get' ctxt, Assertion_SS_Abnormal.get' ctxt))\<close>
 
 \<phi>reasoner_ML assertion_simp 1200
-  (\<open>Simplify (assertion_simps ?ANY) ?X' ?X\<close>)
+  (\<open>Premise (assertion_simps _) _\<close> | \<open>Simplify (assertion_simps ?ANY) ?X' ?X\<close>
+     )
   = \<open>PLPR_Simplifier.simplifier_by_ss' NONE Assertion_SS.get'\<close>
 
 lemmas [assertion_simps] =
