Phi_Test/PhiTest_Aggregate.thy
@@ -2,6 +2,7 @@ theory PhiTest_Aggregate
   imports Phi_Semantics.PhiSem_Aggregate_Array
           Phi_Semantics.PhiSem_Aggregate_Tuple
           Phi_Semantics.PhiSem_CF_Routine
+          Phi_Semantics.PhiSem_CF_Breakable
           Phi_Semantics.PhiSem_Variable
           Phi_Semantics.PhiSem_Int_ArbiPrec
 begin
@@ -11,6 +12,14 @@ no_notation inter (infixl "Int" 70)
         and Nats  ("\<nat>")
         and Ints  ("\<int>")
 
+declare [[\<phi>trace_reasoning =3]]
+
+proc
+  input \<open>(x,y,(z1,z2)) \<Ztypecolon> \<v>\<a>\<l> \<lbrace> \<nat> , \<int> , \<lbrace> \<nat>, \<int> \<rbrace> \<rbrace>\<heavy_comma> aa \<Ztypecolon> \<v>\<a>\<l> \<nat>\<close>
+  output \<open>z1 \<Ztypecolon> \<v>\<a>\<l> \<nat>\<close>   
+  \<medium_left_bracket> op_set_aggregate 0
+    op_get_aggregate 2,0 \<medium_right_bracket>. .
+  
 proc
   input \<open>\<v>\<a>\<l> x \<Ztypecolon> \<nat>\<close>
   premises \<open>x < 10\<close>
